theories/RTac/First.v
@@ -11,11 +11,12 @@ Section parameterized.
   Variable expr : Type.
   Variable subst : Type.
 
-  Variable RType_typ : RType typ.
-  Variable Expr_expr : Expr RType_typ expr.
-  Variable Typ0_Prop : Typ0 _ Prop.
-  Variable Subst_subst : Subst subst expr.
-  Variable SubstOk_subst : @SubstOk _ _ _ _ Expr_expr Subst_subst.
+  Context {RType_typ : RType typ}.
+  Context {Expr_expr : Expr RType_typ expr}.
+  Context {Typ0_Prop : Typ0 _ Prop}.
+  Context {Subst_subst : Subst subst expr}.
+  Context {SubstUpdate_subst : SubstUpdate subst expr}.
+  Context {SubstOk_subst : @SubstOk _ _ _ _ Expr_expr Subst_subst}.
 
   Fixpoint FIRST (tacs : list (rtac typ expr subst))
   : rtac typ expr subst :=
@@ -37,8 +38,7 @@ Section parameterized.
     { unfold rtac_sound. intros; subst; simpl; auto. }
     { red. intros.
       specialize (H ctx s g _ eq_refl).
-      subst. destruct (x ctx s g); eauto.
-      eapply IHForall; reflexivity. }
+      subst. destruct (x ctx s g); eauto. }
   Qed.
 
 End parameterized.
